code/nist-pcurves/Hacl.Impl.P256.Bignum.fsti
@@ -8,53 +8,50 @@ module ST = FStar.HyperStack.ST
 open Lib.IntTypes
 open Lib.Buffer
 
+module S = Spec.P256
 module LSeq = Lib.Sequence
 module BSeq = Lib.ByteSequence
 module BD = Hacl.Spec.Bignum.Definitions
 
 #set-options "--z3rlimit 50 --fuel 0 --ifuel 0"
 
-type curve_t =
-  | P256
-  | P384
-  | P512 
 inline_for_extraction
-let felem = lbuffer uint64 (size 4)
+let felem {| cp:S.curve_params |} = lbuffer uint64 cp.bn_limbs
 inline_for_extraction
-let widefelem = lbuffer uint64 (size 8)
+let widefelem {| cp:S.curve_params |} = lbuffer uint64 (2ul *. cp.bn_limbs)
 
 unfold
-let as_nat (h:mem) (e:felem) : GTot nat =
+let as_nat {| c:S.curve_params |} (h:mem) (e:felem) : GTot nat =
   BD.bn_v (as_seq h e)
 
 unfold
-let wide_as_nat (h:mem) (e:widefelem) : GTot nat =
+let wide_as_nat {| S.curve_params |} (h:mem) (e:widefelem) : GTot nat =
   BD.bn_v (as_seq h e)
 
-val bn_v_is_as_nat: a:LSeq.lseq uint64 4 ->
+val bn_v_is_as_nat4: a:LSeq.lseq uint64 4 ->
   Lemma (let (s0, s1, s2, s3) = LSeq.(a.[0], a.[1], a.[2], a.[3]) in
     BD.bn_v a == v s0 + v s1 * pow2 64 + v s2 * pow2 128 + v s3 * pow2 192)
 
 ///  Create a bignum
 
 inline_for_extraction noextract
-val create_felem: unit -> StackInline felem
+val create_felem: {| c:S.curve_params |} -> StackInline felem
   (requires fun h -> True)
   (ensures  fun h0 f h1 ->
-    stack_allocated f h0 h1 (LSeq.create 4 (u64 0)) /\
+    stack_allocated f h0 h1 (LSeq.create (v c.bn_limbs) (u64 0)) /\
     as_nat h1 f == 0)
 
 
 inline_for_extraction noextract
-val create_widefelem: unit -> StackInline widefelem
+val create_widefelem: {| c:S.curve_params |} -> StackInline widefelem
   (requires fun h -> True)
   (ensures  fun h0 f h1 ->
-    stack_allocated f h0 h1 (LSeq.create 8 (u64 0)) /\
+    stack_allocated f h0 h1 (LSeq.create (2 * v c.bn_limbs) (u64 0)) /\
     wide_as_nat h1 f == 0)
 
 
 inline_for_extraction noextract
-val bn_make_u64_4: res:felem -> a0:uint64 -> a1:uint64 -> a2:uint64 -> a3:uint64 -> Stack unit
+val bn_make_u64_4: {| c:S.curve_params |} -> res:felem -> a0:uint64 -> a1:uint64 -> a2:uint64 -> a3:uint64{c.bn_limbs == 4ul} -> Stack unit
   (requires fun h -> live h res)
   (ensures  fun h0 _ h1 -> modifies (loc res) h0 h1 /\
     as_nat h1 res = v a0 + v a1 * pow2 64 + v a2 * pow2 128 + v a3 * pow2 192)
@@ -63,14 +60,14 @@ val bn_make_u64_4: res:felem -> a0:uint64 -> a1:uint64 -> a2:uint64 -> a3:uint64
 ///  Create zero and one
 
 inline_for_extraction noextract
-val bn_set_zero4: f:felem -> Stack unit
+val bn_set_zero: {| c:S.curve_params |} -> f:felem -> Stack unit
   (requires fun h -> live h f)
   (ensures fun h0 _ h1 -> modifies (loc f) h0 h1 /\
     as_nat h1 f == 0)
 
 
 inline_for_extraction noextract
-val bn_set_one4: f:felem -> Stack unit
+val bn_set_one: {| c:S.curve_params |} -> f:felem -> Stack unit
   (requires fun h -> live h f)
   (ensures fun h0 _ h1 -> modifies (loc f) h0 h1 /\
     as_nat h1 f == 1)
@@ -78,31 +75,31 @@ val bn_set_one4: f:felem -> Stack unit
 
 ///  Comparison
 
-val bn_is_zero_mask4: f:felem -> Stack uint64
+val bn_is_zero_mask: {| c:S.curve_params |} ->  f:felem -> Stack uint64
   (requires fun h -> live h f)
   (ensures fun h0 r h1 -> modifies0 h0 h1 /\
     (if as_nat h0 f = 0 then v r == ones_v U64 else v r == 0))
 
 
-val bn_is_zero_vartime4: f:felem -> Stack bool
+val bn_is_zero_vartime: {| c:S.curve_params |} -> f:felem -> Stack bool
   (requires fun h -> live h f)
   (ensures fun h0 r h1 -> modifies0 h0 h1 /\ r == (as_nat h0 f = 0))
 
 
-val bn_is_eq_mask4: x:felem -> y:felem -> Stack uint64
+val bn_is_eq_mask: {| c:S.curve_params |} -> x:felem -> y:felem -> Stack uint64
   (requires fun h -> live h x /\ live h y)
   (ensures fun h0 r h1 -> modifies0 h0 h1 /\
     (if as_nat h0 x = as_nat h0 y then v r == ones_v U64 else v r = 0))
 
 
-val bn_is_eq_vartime4: x:felem -> y:felem -> Stack bool
+val bn_is_eq_vartime: {| c:S.curve_params |} -> x:felem -> y:felem -> Stack bool
   (requires fun h -> live h x /\ live h y)
   (ensures  fun h0 r h1 -> modifies0 h0 h1 /\
     r == (as_nat h0 x = as_nat h0 y))
 
 
 inline_for_extraction noextract
-val bn_is_odd4: f:felem -> Stack uint64
+val bn_is_odd: {| c:S.curve_params |} -> f:felem -> Stack uint64
   (requires fun h -> live h f)
   (ensures  fun h0 r h1 -> modifies0 h0 h1 /\
     v r = (as_nat h0 f % 2))
@@ -110,7 +107,7 @@ val bn_is_odd4: f:felem -> Stack uint64
 
 ///  Conditional copy
 
-val bn_cmovznz4: res:felem -> cin:uint64 -> x:felem -> y:felem -> Stack unit
+val bn_cmovznz: {| c:S.curve_params |} -> res:felem -> cin:uint64 -> x:felem -> y:felem -> Stack unit
   (requires fun h ->
     live h x /\ live h y /\ live h res /\
     eq_or_disjoint res x /\ eq_or_disjoint res y /\ eq_or_disjoint x y)
@@ -120,7 +117,7 @@ val bn_cmovznz4: res:felem -> cin:uint64 -> x:felem -> y:felem -> Stack unit
 
 ///  Addition and subtraction
 
-val bn_add_mod4: res:felem -> n:felem -> x:felem -> y:felem -> Stack unit
+val bn_add_mod: {| c:S.curve_params |} -> res:felem -> n:felem -> x:felem -> y:felem -> Stack unit
   (requires fun h ->
     live h n /\ live h x /\ live h y /\ live h res /\
     disjoint n x /\ disjoint n y /\ disjoint n res /\
@@ -130,16 +127,16 @@ val bn_add_mod4: res:felem -> n:felem -> x:felem -> y:felem -> Stack unit
     as_nat h1 res == (as_nat h0 x + as_nat h0 y) % as_nat h0 n)
 
 
-val bn_sub4: res:felem -> x:felem -> y:felem -> Stack uint64
+val bn_sub: {| cp:S.curve_params |} -> res:felem -> x:felem -> y:felem -> Stack uint64
   (requires fun h ->
     live h x /\ live h y /\ live h res /\
     eq_or_disjoint x y /\ eq_or_disjoint x res /\ eq_or_disjoint y res)
   (ensures fun h0 c h1 -> modifies (loc res) h0 h1 /\ v c <= 1 /\
-    as_nat h1 res - v c * pow2 256 == as_nat h0 x - as_nat h0 y /\
+    as_nat h1 res - v c * pow2 cp.bits == as_nat h0 x - as_nat h0 y /\
     (if v c = 0 then as_nat h0 x >= as_nat h0 y else as_nat h0 x < as_nat h0 y))
 
 
-val bn_sub_mod4: res:felem -> n:felem -> x:felem -> y:felem -> Stack unit
+val bn_sub_mod: {| c:S.curve_params |} -> res:felem -> n:felem -> x:felem -> y:felem -> Stack unit
   (requires fun h ->
     live h n /\ live h x /\ live h y /\ live h res /\
     disjoint n x /\ disjoint n y /\ disjoint n res /\
@@ -151,7 +148,7 @@ val bn_sub_mod4: res:felem -> n:felem -> x:felem -> y:felem -> Stack unit
 
 ///  Multiplication
 
-val bn_mul4: res:widefelem -> x:felem -> y:felem -> Stack unit
+val bn_mul: {| c:S.curve_params |} -> res:widefelem -> x:felem -> y:felem -> Stack unit
   (requires fun h ->
     live h res /\ live h x /\ live h y /\
     eq_or_disjoint x y /\ disjoint x res /\ disjoint y res)
@@ -159,7 +156,7 @@ val bn_mul4: res:widefelem -> x:felem -> y:felem -> Stack unit
     wide_as_nat h1 res = as_nat h0 x * as_nat h0 y)
 
 
-val bn_sqr4: res:widefelem -> x:felem -> Stack unit
+val bn_sqr: {| c:S.curve_params |} -> res:widefelem -> x:felem -> Stack unit
   (requires fun h ->
     live h res /\ live h x /\ eq_or_disjoint x res)
   (ensures  fun h0 _ h1 -> modifies (loc res) h0 h1 /\
@@ -168,25 +165,25 @@ val bn_sqr4: res:widefelem -> x:felem -> Stack unit
 
 ///  Conversion between bignum and bytes representation
 
-val bn_to_bytes_be4: res:lbuffer uint8 32ul -> f:felem -> Stack unit
+val bn_to_bytes_be: {| c:S.curve_params |} -> res:lbuffer uint8 (size c.bytes) -> f:felem -> Stack unit
   (requires fun h ->
     live h f /\ live h res /\ disjoint f res /\
-    as_nat h f < pow2 256)
+    as_nat h f < pow2 (8 * c.bytes))
   (ensures fun h0 _ h1 -> modifies (loc res) h0 h1 /\
-    as_seq h1 res == BSeq.nat_to_bytes_be 32 (as_nat h0 f))
+    as_seq h1 res == BSeq.nat_to_bytes_be c.bytes (as_nat h0 f))
 
 
-val bn_from_bytes_be4: res:felem -> b:lbuffer uint8 32ul -> Stack unit
+val bn_from_bytes_be: {| c:S.curve_params |} -> res:felem -> b:lbuffer uint8 (size c.bytes) -> Stack unit
   (requires fun h -> live h b /\ live h res /\ disjoint b res)
   (ensures  fun h0 _ h1 -> modifies (loc res) h0 h1 /\
     as_nat h1 res == BSeq.nat_from_bytes_be (as_seq h0 b))
 
 
-val bn2_to_bytes_be4: res:lbuffer uint8 64ul -> x:felem -> y:felem -> Stack unit
+val bn2_to_bytes_be: {| c:S.curve_params |} -> res:lbuffer uint8 (2ul *. size c.bytes) -> x:felem -> y:felem -> Stack unit
   (requires fun h ->
     live h x /\ live h y /\ live h res /\
     disjoint x res /\ disjoint y res /\
-    as_nat h x < pow2 256 /\ as_nat h y < pow2 256)
+    as_nat h x < pow2 (8*c.bytes) /\ as_nat h y < pow2 (8*c.bytes))
   (ensures fun h0 _ h1 -> modifies (loc res) h0 h1 /\
-    as_seq h1 res == LSeq.concat #uint8 #32 #32
-      (BSeq.nat_to_bytes_be 32 (as_nat h0 x)) (BSeq.nat_to_bytes_be 32 (as_nat h0 y)))
+    as_seq h1 res == LSeq.concat #uint8 #c.bytes #c.bytes
+      (BSeq.nat_to_bytes_be c.bytes (as_nat h0 x)) (BSeq.nat_to_bytes_be c.bytes (as_nat h0 y)))
