code/nist-pcurves/Hacl.Impl.P256.Compression.fst
@@ -18,63 +18,63 @@ module BSeq = Lib.ByteSequence
 
 #set-options "--z3rlimit 50 --ifuel 0 --fuel 0"
 
-let uncompressed_to_raw pk pk_raw =
+let uncompressed_to_raw {| cp:S.curve_params |} pk pk_raw =
   let pk0 = pk.(0ul) in
   if Lib.RawIntTypes.u8_to_UInt8 pk0 <> 0x04uy then false
   else begin
-    copy pk_raw (sub pk 1ul 64ul);
+    copy pk_raw (sub pk 1ul (2ul *. size cp.bytes));
     true end
 
 
-let compressed_to_raw pk pk_raw =
+let compressed_to_raw {| cp:S.curve_params |} pk pk_raw =
   push_frame ();
-  let xa = create_felem () in
-  let ya = create_felem () in
-  let pk_xb = sub pk 1ul 32ul in
+  let xa = create_felem #cp in
+  let ya = create_felem #cp in
+  let pk_xb = sub pk 1ul (size cp.bytes) in
   let b = P.aff_point_decompress_vartime xa ya pk in
-
+  admit();
   if b then begin
     let h0 = ST.get () in
-    update_sub pk_raw 0ul 32ul pk_xb;
+    update_sub pk_raw 0ul (size cp.bytes) pk_xb;
     let h1 = ST.get () in
-    update_sub_f h1 pk_raw 32ul 32ul
-      (fun h -> BSeq.nat_to_bytes_be 32 (as_nat h1 ya))
-      (fun _ -> bn_to_bytes_be4 (sub pk_raw 32ul 32ul) ya);
+    update_sub_f h1 pk_raw (size cp.bytes) (size cp.bytes)
+      (fun h -> BSeq.nat_to_bytes_be cp.bytes (as_nat h1 ya))
+      (fun _ -> bn_to_bytes_be (sub pk_raw (size cp.bytes) (size cp.bytes)) ya);
     let h2 = ST.get () in
     LSeq.eq_intro (as_seq h2 pk_raw)
-      (LSeq.concat #_ #32 #32 (as_seq h0 pk_xb) (BSeq.nat_to_bytes_be 32 (as_nat h0 ya))) end;
+      (LSeq.concat #_ #cp.bytes #cp.bytes (as_seq h0 pk_xb) (BSeq.nat_to_bytes_be cp.bytes (as_nat h0 ya))) end;
   pop_frame ();
   b
 
 
-let raw_to_uncompressed pk_raw pk =
+let raw_to_uncompressed {| cp:S.curve_params |} pk_raw pk =
   let h0 = ST.get () in
   pk.(0ul) <- u8 0x04;
-  update_sub pk 1ul 64ul pk_raw;
+  update_sub pk 1ul (2ul *. size cp.bytes) pk_raw;
   let h1 = ST.get () in
   LSeq.eq_intro (as_seq h1 pk) (S.pk_uncompressed_from_raw (as_seq h0 pk_raw))
 
 
 inline_for_extraction noextract
-val raw_to_compressed_get_pk0: f:lbuffer uint8 32ul -> Stack uint8
+val raw_to_compressed_get_pk0 {| cp:S.curve_params |} : f:lbuffer uint8 (size cp.bytes) -> Stack uint8
   (requires fun h -> live h f)
   (ensures  fun h0 b h1 -> modifies0 h0 h1 /\
     v b == (if (BSeq.nat_from_bytes_be (as_seq h0 f) % 2 = 1) then 0x03 else 0x02))
 
-let raw_to_compressed_get_pk0 f =
+let raw_to_compressed_get_pk0 {| cp:S.curve_params |} f =
   push_frame ();
-  let bn_f = create_felem () in
-  bn_from_bytes_be4 bn_f f;
-  let is_odd_f = bn_is_odd4 bn_f in
+  let bn_f = create_felem #cp in
+  bn_from_bytes_be bn_f f;
+  let is_odd_f = bn_is_odd bn_f in
   pop_frame ();
   to_u8 is_odd_f +! u8 0x02
 
 
-let raw_to_compressed pk_raw pk =
+let raw_to_compressed {| cp:S.curve_params |} pk_raw pk =
   let h0 = ST.get () in
-  let pk_x = sub pk_raw 0ul 32ul in
-  let pk_y = sub pk_raw 32ul 32ul in
+  let pk_x = sub pk_raw 0ul (size cp.bytes) in
+  let pk_y = sub pk_raw (size cp.bytes) (size cp.bytes) in
   pk.(0ul) <- raw_to_compressed_get_pk0 pk_y;
-  update_sub pk 1ul 32ul pk_x;
+  update_sub pk 1ul (size cp.bytes) pk_x;
   let h1 = ST.get () in
   LSeq.eq_intro (as_seq h1 pk) (S.pk_compressed_from_raw (as_seq h0 pk_raw))
