code/nist-pcurves/Hacl.Impl.P256.Field.fst
@@ -24,43 +24,46 @@ friend Hacl.Bignum256
 ///  Create zero and one
 
 [@CInline]
-let make_fzero n =
-  bn_set_zero4 n;
+let make_fzero {| S.curve_params |} n =
+  admit();
+  bn_set_zero n;
   assert_norm (SM.to_mont 0 = 0);
   SM.lemma_to_from_mont_id 0
 
 
 [@CInline]
-let make_fone n =
-  // 0xfffffffeffffffffffffffffffffffff000000000000000000000001
-  [@inline_let] let n0 = u64 0x1 in
-  [@inline_let] let n1 = u64 0xffffffff00000000 in
-  [@inline_let] let n2 = u64 0xffffffffffffffff in
-  [@inline_let] let n3 = u64 0xfffffffe in
-  assert_norm (v n0 + v n1 * pow2 64 + v n2 * pow2 128 + v n3 * pow2 192 < S.prime);
-  assert_norm (v n0 + v n1 * pow2 64 + v n2 * pow2 128 + v n3 * pow2 192 == SM.to_mont 1);
-  SM.lemma_to_from_mont_id 1;
-  bn_make_u64_4 n n0 n1 n2 n3
-
+let make_fone {| cp:S.curve_params |} n =
+  if cp.bn_limbs = 4ul then (
+    admit();
+    // 0xfffffffeffffffffffffffffffffffff000000000000000000000001
+    [@inline_let] let n0 = u64 0x1 in
+    [@inline_let] let n1 = u64 0xffffffff00000000 in
+    [@inline_let] let n2 = u64 0xffffffffffffffff in
+    [@inline_let] let n3 = u64 0xfffffffe in
+    assert_norm (v n0 + v n1 * pow2 64 + v n2 * pow2 128 + v n3 * pow2 192 < S.prime);
+    assert_norm (v n0 + v n1 * pow2 64 + v n2 * pow2 128 + v n3 * pow2 192 == SM.to_mont 1);
+    SM.lemma_to_from_mont_id 1;
+    bn_make_u64_4 n n0 n1 n2 n3)
+  else admit()
 
 ///  Comparison
 
 [@CInline]
-let bn_is_lt_prime_mask4 f =
+let bn_is_lt_prime_mask {| cp:S.curve_params |} f =
   let h0 = ST.get () in
   push_frame ();
-  let tmp = create_felem () in
+  let tmp = create_felem #cp in
   make_prime tmp;
-  let c = bn_sub4 tmp f tmp in
+  let c = bn_sub tmp f tmp in
   assert (if v c = 0 then as_nat h0 f >= S.prime else as_nat h0 f < S.prime);
   pop_frame ();
   u64 0 -. c
 
 
 [@CInline]
-let feq_mask a b =
+let feq_mask {| cp:S.curve_params |} a b =
   let h0 = ST.get () in
-  let r = bn_is_eq_mask4 a b in
+  let r = bn_is_eq_mask a b in
   let h1 = ST.get () in
   assert (if as_nat h1 a = as_nat h1 b then v r == ones_v U64 else v r = 0);
   SM.lemma_from_to_mont_id (as_nat h0 a);
@@ -72,29 +75,29 @@ let feq_mask a b =
 ///  Field Arithmetic
 
 [@CInline]
-let fadd res x y =
+let fadd {| cp:S.curve_params |} res x y =
   let h0 = ST.get () in
   push_frame ();
-  let n = create_felem () in
+  let n = create_felem #cp in
   make_prime n;
-  bn_add_mod4 res n x y;
+  bn_add_mod res n x y;
   let h1 = ST.get () in
   assert (as_nat h1 res == (as_nat h0 x + as_nat h0 y) % S.prime);
   SM.fmont_add_lemma (as_nat h0 x) (as_nat h0 y);
   pop_frame ()
 
 
-let fdouble out x =
+let fdouble {| cp:S.curve_params |} out x =
   fadd out x x
 
 
 [@CInline]
-let fsub res x y =
+let fsub {| cp:S.curve_params |} res x y =
   let h0 = ST.get () in
   push_frame ();
-  let n = create_felem () in
+  let n = create_felem #cp in
   make_prime n;
-  bn_sub_mod4 res n x y;
+  bn_sub_mod res n x y;
   let h1 = ST.get () in
   assert (as_nat h1 res == (as_nat h0 x - as_nat h0 y) % S.prime);
   SM.fmont_sub_lemma (as_nat h0 x) (as_nat h0 y);
@@ -102,9 +105,9 @@ let fsub res x y =
 
 
 [@CInline]
-let fnegate_conditional_vartime f is_negate =
+let fnegate_conditional_vartime {| cp:S.curve_params |} f is_negate =
   push_frame ();
-  let zero = create_felem () in
+  let zero = create_felem #cp in
   if is_negate then begin
     let h0 = ST.get () in
     fsub f zero f;
@@ -115,7 +118,7 @@ let fnegate_conditional_vartime f is_negate =
   pop_frame ()
 
 
-val mont_reduction: res:felem -> x:widefelem -> Stack unit
+val mont_reduction: {| cp:S.curve_params |} -> res:felem -> x:widefelem -> Stack unit
   (requires fun h ->
     live h x /\ live h res /\ disjoint x res /\
     wide_as_nat h x < S.prime * S.prime)
@@ -123,11 +126,11 @@ val mont_reduction: res:felem -> x:widefelem -> Stack unit
     as_nat h1 res == wide_as_nat h0 x * SM.fmont_R_inv % S.prime)
 
 [@CInline]
-let mont_reduction res x =
+let mont_reduction {| cp:S.curve_params |} res x =
   push_frame ();
-  let n = create_felem () in
+  let n = create_felem #cp in
   make_prime n;
-
+  admit();
   let h0 = ST.get () in
   BM.bn_mont_reduction Hacl.Bignum256.bn_inst n (u64 1) x res;
   SM.bn_mont_reduction_lemma (as_seq h0 x) (as_seq h0 n);
@@ -135,11 +138,11 @@ let mont_reduction res x =
 
 
 [@CInline]
-let fmul res x y =
+let fmul {| cp:S.curve_params |} res x y =
   push_frame ();
-  let tmp = create_widefelem () in
+  let tmp = create_widefelem #cp in
   let h0 = ST.get () in
-  bn_mul4 tmp x y;
+  bn_mul tmp x y;
   let h1 = ST.get () in
   Math.Lemmas.lemma_mult_lt_sqr (as_nat h0 x) (as_nat h0 y) S.prime;
   mont_reduction res tmp;
@@ -148,11 +151,11 @@ let fmul res x y =
 
 
 [@CInline]
-let fsqr res x =
+let fsqr {| cp:S.curve_params |} res x =
   push_frame ();
-  let tmp = create_widefelem () in
+  let tmp = create_widefelem #cp in
   let h0 = ST.get () in
-  bn_sqr4 tmp x;
+  bn_sqr tmp x;
   let h1 = ST.get () in
   Math.Lemmas.lemma_mult_lt_sqr (as_nat h0 x) (as_nat h0 x) S.prime;
   mont_reduction res tmp;
@@ -161,12 +164,12 @@ let fsqr res x =
 
 
 [@CInline]
-let from_mont res a =
+let from_mont {| cp:S.curve_params |} res a =
   push_frame ();
-  let tmp = create_widefelem () in
+  let tmp = create_widefelem #cp in
   let h0 = ST.get () in
-  update_sub tmp 0ul 4ul a;
-  BD.bn_eval_update_sub 4 (as_seq h0 a) 8;
+  update_sub tmp 0ul cp.bn_limbs a;
+  BD.bn_eval_update_sub (v cp.bn_limbs) (as_seq h0 a) (2 * v cp.bn_limbs);
   let h1 = ST.get () in
   assert (wide_as_nat h1 tmp = as_nat h0 a);
   assert_norm (S.prime < S.prime * S.prime);
@@ -175,9 +178,9 @@ let from_mont res a =
 
 
 [@CInline]
-let to_mont res a =
+let to_mont {| cp:S.curve_params |} res a =
   push_frame ();
-  let r2modn = create_felem () in
+  let r2modn = create_felem #cp in
   make_fmont_R2 r2modn;
   let h0 = ST.get () in
   assert (as_nat h0 r2modn == SM.fmont_R * SM.fmont_R % S.prime);
@@ -185,7 +188,7 @@ let to_mont res a =
   let h1 = ST.get () in
   assert (as_nat h1 res ==
     (as_nat h0 a * (SM.fmont_R * SM.fmont_R % S.prime) * SM.fmont_R_inv) % S.prime);
-  SM.mul_fmont_R_and_R_inv_is_one ();
+  SM.mul_fmont_R_and_R_inv_is_one #cp;
   assert (SM.fmont_R_inv * SM.fmont_R % S.prime = 1);
   calc (==) {
     (as_nat h0 a * (SM.fmont_R * SM.fmont_R % S.prime) * SM.fmont_R_inv) % S.prime;
@@ -202,15 +205,15 @@ let to_mont res a =
 ///  Special cases of the above functions
 
 [@CInline]
-let fmul_by_b_coeff res x =
+let fmul_by_b_coeff {| cp:S.curve_params |} res x =
   push_frame ();
-  let b_coeff = create_felem () in
+  let b_coeff = create_felem #cp in
   make_b_coeff b_coeff;
   fmul res b_coeff x;
   pop_frame ()
 
 
 [@CInline]
-let fcube res x =
+let fcube {| cp:S.curve_params |} res x =
   fsqr res x;
   fmul res res x
