code/nist-pcurves/Hacl.Impl.P256.Point.fsti
@@ -23,11 +23,11 @@ let from_mont_point {| S.curve_params |} (a:tuple3 nat nat nat) : S.proj_point =
 ///  Affine coordinates
 
 inline_for_extraction noextract
-let aff_point_seq = LSeq.lseq uint64 8
+let aff_point_seq {| cp:S.curve_params |} = LSeq.lseq uint64 (2 * v cp.bn_limbs)
 
-let as_aff_point_nat_seq (p:aff_point_seq) =
-  BD.bn_v (LSeq.sub p 0 4),
-  BD.bn_v (LSeq.sub p 4 4)
+let as_aff_point_nat_seq {| cp:S.curve_params |} (p:aff_point_seq) =
+  BD.bn_v (LSeq.sub p 0 (v cp.bn_limbs)),
+  BD.bn_v (LSeq.sub p (v cp.bn_limbs) (v cp.bn_limbs))
 
 let aff_point_inv_seq {| S.curve_params |} (p:aff_point_seq) =
   let x, y = as_aff_point_nat_seq p in
@@ -35,10 +35,10 @@ let aff_point_inv_seq {| S.curve_params |} (p:aff_point_seq) =
 
 
 inline_for_extraction noextract
-let aff_point = lbuffer uint64 8ul
+let aff_point {| cp:S.curve_params |} = lbuffer uint64 (2ul *. S.bn_limbs)
 
 noextract
-let as_aff_point_nat (h:mem) (p:aff_point) =
+let as_aff_point_nat {| cp:S.curve_params |} (h:mem) (p:aff_point) =
   as_aff_point_nat_seq (as_seq h p)
 
 noextract
@@ -46,46 +46,52 @@ let aff_point_inv {| S.curve_params |} (h:mem) (p:aff_point) =
   aff_point_inv_seq (as_seq h p)
 
 noextract
-let aff_point_x_as_nat (h:mem) (p:aff_point) : GTot nat =
-  as_nat h (gsub p 0ul 4ul)
+let as_aff_point_nat_inv {| cp:S.curve_params |} (h:mem) (p:aff_point{aff_point_inv h p}) : GTot S.aff_point  =
+  let (x,y)= as_aff_point_nat h p in (x,y)
 
 noextract
-let aff_point_y_as_nat (h:mem) (p:aff_point) : GTot nat =
-  as_nat h (gsub p 4ul 4ul)
+let aff_point_x_as_nat {| cp:S.curve_params |} (h:mem) (p:aff_point) : GTot nat =
+  as_nat h (gsub p 0ul cp.bn_limbs)
+
+noextract
+let aff_point_y_as_nat {| cp:S.curve_params |} (h:mem) (p:aff_point) : GTot nat =
+  as_nat h (gsub p cp.bn_limbs cp.bn_limbs)
 
 inline_for_extraction noextract
-let aff_getx (p:aff_point) : Stack felem
+let aff_getx {| cp:S.curve_params |} (p:aff_point) : Stack felem
   (requires fun h -> live h p)
-  (ensures fun h0 f h1 -> f == gsub p 0ul 4ul /\ h0 == h1)
-  = sub p 0ul 4ul
+  (ensures fun h0 f h1 -> f == gsub p 0ul cp.bn_limbs /\ h0 == h1)
+  = sub p 0ul cp.bn_limbs
 
 inline_for_extraction noextract
-let aff_gety (p:aff_point) : Stack felem
+let aff_gety {| cp:S.curve_params |} (p:aff_point) : Stack felem
   (requires fun h -> live h p)
-  (ensures fun h0 f h1 -> f == gsub p 4ul 4ul /\ h0 == h1)
-  = sub p 4ul 4ul
+  (ensures fun h0 f h1 -> f == gsub p cp.bn_limbs cp.bn_limbs /\ h0 == h1)
+  = sub p cp.bn_limbs cp.bn_limbs
 
 
 ///  Projective coordinates
 
 inline_for_extraction noextract
-let point_seq = LSeq.lseq uint64 12
+let point_seq {| cp:S.curve_params |} = LSeq.lseq uint64 (3 * v cp.bn_limbs)
 
-let as_point_nat_seq (p:point_seq) =
-  BD.bn_v (LSeq.sub p 0 4),
-  BD.bn_v (LSeq.sub p 4 4),
-  BD.bn_v (LSeq.sub p 8 4)
+noextract
+let as_point_nat_seq {| cp:S.curve_params |} (p:point_seq) =
+  BD.bn_v (LSeq.sub p 0 (v cp.bn_limbs)),
+  BD.bn_v (LSeq.sub p (v cp.bn_limbs) (v cp.bn_limbs)),
+  BD.bn_v (LSeq.sub p (2 * v cp.bn_limbs) (v cp.bn_limbs))
 
+noextract
 let point_inv_seq {| S.curve_params |} (p:point_seq) =
   let x, y, z = as_point_nat_seq p in
   x < S.prime /\ y < S.prime /\ z < S.prime
 
 
 inline_for_extraction noextract
-let point = lbuffer uint64 12ul
+let point {| cp:S.curve_params |} = lbuffer uint64 (3ul *. cp.bn_limbs)
 
 noextract
-let as_point_nat (h:mem) (p:point) =
+let as_point_nat {| cp:S.curve_params |} (h:mem) (p:point) =
   as_point_nat_seq (as_seq h p)
 
 noextract
@@ -93,51 +99,55 @@ let point_inv {| S.curve_params |} (h:mem) (p:point) =
   point_inv_seq (as_seq h p)
 
 noextract
-let point_x_as_nat (h:mem) (p:point) : GTot nat =
-  as_nat h (gsub p 0ul 4ul)
+let as_point_nat_inv {| cp:S.curve_params |} (h:mem) (p:point{point_inv h p}) : GTot S.proj_point =
+  let (x,y,z) = as_point_nat h p  in (x,y,z)
 
 noextract
-let point_y_as_nat (h:mem) (e:point) : GTot nat =
-  as_nat h (gsub e 4ul 4ul)
+let point_x_as_nat {| cp:S.curve_params |} (h:mem) (p:point) : GTot nat =
+  as_nat h (gsub p 0ul cp.bn_limbs)
 
 noextract
-let point_z_as_nat (h:mem) (e:point) : GTot nat =
-  as_nat h (gsub e 8ul 4ul)
+let point_y_as_nat {| cp:S.curve_params |} (h:mem) (e:point) : GTot nat =
+  as_nat h (gsub e cp.bn_limbs cp.bn_limbs)
+
+noextract
+let point_z_as_nat {| cp:S.curve_params |} (h:mem) (e:point) : GTot nat =
+  as_nat h (gsub e (2ul *. cp.bn_limbs) (cp.bn_limbs))
 
 
 inline_for_extraction noextract
-let getx (p:point) : Stack felem
+let getx {| cp:S.curve_params |} (p:point) : Stack felem
   (requires fun h -> live h p)
-  (ensures fun h0 f h1 -> f == gsub p 0ul 4ul /\ h0 == h1)
-  = sub p 0ul 4ul
+  (ensures fun h0 f h1 -> f == gsub p 0ul cp.bn_limbs /\ h0 == h1)
+  = sub p 0ul cp.bn_limbs
 
 inline_for_extraction noextract
-let gety (p:point) : Stack felem
+let gety {| cp:S.curve_params |} (p:point) : Stack felem
   (requires fun h -> live h p)
-  (ensures fun h0 f h1 -> f == gsub p 4ul 4ul /\ h0 == h1)
-  = sub p 4ul 4ul
+  (ensures fun h0 f h1 -> f == gsub p cp.bn_limbs cp.bn_limbs /\ h0 == h1)
+  = sub p cp.bn_limbs cp.bn_limbs
 
 inline_for_extraction noextract
-let getz (p:point) : Stack felem
+let getz {| cp:S.curve_params |} (p:point) : Stack felem
   (requires fun h -> live h p)
-  (ensures fun h0 f h1 -> f == gsub p 8ul 4ul /\ h0 == h1)
-  = sub p 8ul 4ul
+  (ensures fun h0 f h1 -> f == gsub p (2ul *. cp.bn_limbs) (cp.bn_limbs) /\ h0 == h1)
+  = sub p (2ul *. cp.bn_limbs) (cp.bn_limbs)
 
 
 ///  Create a point
 
 inline_for_extraction noextract
-val create_aff_point: unit -> StackInline aff_point
+val create_aff_point: {| cp:S.curve_params |} -> StackInline aff_point
   (requires fun h -> True)
   (ensures  fun h0 f h1 ->
-    stack_allocated f h0 h1 (LSeq.create 8 (u64 0)))
+    stack_allocated f h0 h1 (LSeq.create (2 * v cp.bn_limbs) (u64 0)))
 
 
 inline_for_extraction noextract
-val create_point: unit -> StackInline point
+val create_point: {| cp:S.curve_params |} -> StackInline point
   (requires fun h -> True)
   (ensures  fun h0 f h1 ->
-    stack_allocated f h0 h1 (LSeq.create 12 (u64 0)))
+    stack_allocated f h0 h1 (LSeq.create (3 * v cp.bn_limbs) (u64 0)))
 
 
 val make_base_point: {| S.curve_params |} -> p:point -> Stack unit
@@ -159,20 +169,20 @@ val is_point_at_inf: {| S.curve_params |} -> p:point -> Stack uint64
   (ensures fun h0 r h1 -> modifies0 h0 h1 /\
     (let pM = from_mont_point (as_point_nat h0 p) in
     (if S.is_point_at_inf pM then v r = ones_v U64 else v r = 0) /\
-    (if S.is_point_at_inf (as_point_nat h0 p) then v r = ones_v U64 else v r = 0)))
+    (if S.is_point_at_inf (as_point_nat_inv h0 p) then v r = ones_v U64 else v r = 0)))
 
 
-val is_point_at_inf_vartime: p:point -> Stack bool
+val is_point_at_inf_vartime: {| S.curve_params |} -> p:point -> Stack bool
   (requires fun h -> live h p /\ point_inv h p)
   (ensures  fun h0 r h1 -> modifies0 h0 h1 /\
-    r == S.is_point_at_inf (as_point_nat h0 p) /\
+    r == S.is_point_at_inf (as_point_nat_inv h0 p) /\
     r == S.is_point_at_inf (from_mont_point (as_point_nat h0 p)))
 
 
 ///  Create a copy of a point
 
 inline_for_extraction noextract
-val copy_point: res:point -> p:point -> Stack unit
+val copy_point: {| S.curve_params |} -> res:point -> p:point -> Stack unit
   (requires fun h -> live h p /\ live h res /\ disjoint p res)
   (ensures fun h0 _ h1 -> modifies (loc res) h0 h1 /\
     as_seq h1 res == as_seq h0 p)
@@ -181,16 +191,17 @@ val copy_point: res:point -> p:point -> Stack unit
 ///  Point conversion between Projective and Affine coordinates representations
 
 // to_aff_point = S.to_aff_point + from_mont
-val to_aff_point: res:aff_point -> p:point -> Stack unit
+val to_aff_point: {| S.curve_params |} -> res:aff_point -> p:point -> Stack unit
   (requires fun h ->
     live h p /\ live h res /\ eq_or_disjoint p res /\
     point_inv h p)
   (ensures fun h0 _ h1 -> modifies (loc res) h0 h1 /\
-    as_aff_point_nat h1 res == S.to_aff_point (from_mont_point (as_point_nat h0 p)))
+    aff_point_inv h1 res /\
+    as_aff_point_nat_inv h1 res == S.to_aff_point (from_mont_point (as_point_nat h0 p)))
 
 
 // to_aff_point = S.to_aff_point + from_mont
-val to_aff_point_x: res:felem -> p:point -> Stack unit
+val to_aff_point_x: {| S.curve_params |} -> res:felem -> p:point -> Stack unit
   (requires fun h ->
     live h p /\ live h res /\ eq_or_disjoint p res /\
     point_inv h p)
@@ -199,34 +210,34 @@ val to_aff_point_x: res:felem -> p:point -> Stack unit
 
 
 // to_proj_point = S.to_proj_point + to_mont
-val to_proj_point: res:point -> p:aff_point -> Stack unit
+val to_proj_point: {| S.curve_params |} -> res:point -> p:aff_point -> Stack unit
   (requires fun h ->
     live h p /\ live h res /\ disjoint p res /\
     aff_point_inv h p)
   (ensures  fun h0 _ h1 -> modifies (loc res) h0 h1 /\
     point_inv h1 res /\
-    from_mont_point (as_point_nat h1 res) == S.to_proj_point (as_aff_point_nat h0 p))
+    from_mont_point (as_point_nat h1 res) == S.to_proj_point (as_aff_point_nat_inv h0 p))
 
 
 ///  Check if a point is on the curve
 
-val is_on_curve_vartime: p:aff_point -> Stack bool
+val is_on_curve_vartime: {| S.curve_params |} -> p:aff_point -> Stack bool
   (requires fun h -> live h p /\ aff_point_inv h p)
   (ensures fun h0 r h1 -> modifies0 h0 h1 /\
-    r == S.is_on_curve (as_aff_point_nat h0 p))
+    r == S.is_on_curve (as_aff_point_nat_inv h0 p))
 
 
 ///  Point load and store functions
 
-val aff_point_store: res:lbuffer uint8 64ul -> p:aff_point -> Stack unit
+val aff_point_store: {| S.curve_params |} -> res:lbuffer uint8 64ul -> p:aff_point -> Stack unit
   (requires fun h ->
     live h res /\ live h p /\ disjoint res p /\
     aff_point_inv h p)
   (ensures  fun h0 _ h1 -> modifies (loc res) h0 h1 /\
-    as_seq h1 res == S.aff_point_store (as_aff_point_nat h0 p))
+    as_seq h1 res == S.aff_point_store (as_aff_point_nat_inv h0 p))
 
 
-val point_store: res:lbuffer uint8 64ul -> p:point -> Stack unit
+val point_store: {| S.curve_params |} -> res:lbuffer uint8 64ul -> p:point -> Stack unit
   (requires fun h ->
     live h res /\ live h p /\ disjoint res p /\
     point_inv h p)
@@ -234,15 +245,15 @@ val point_store: res:lbuffer uint8 64ul -> p:point -> Stack unit
     as_seq h1 res == S.point_store (from_mont_point (as_point_nat h0 p)))
 
 
-val aff_point_load_vartime: res:aff_point -> b:lbuffer uint8 64ul -> Stack bool
+val aff_point_load_vartime: {| cp:S.curve_params |} -> res:aff_point -> b:lbuffer uint8 (2ul *. size cp.bytes) -> Stack bool
   (requires fun h ->
     live h res /\ live h b /\ disjoint res b)
   (ensures  fun h0 r h1 -> modifies (loc res) h0 h1 /\
     (let ps = S.aff_point_load (as_seq h0 b) in
-    (r <==> Some? ps) /\ (r ==> (aff_point_inv h1 res /\ as_aff_point_nat h1 res == Some?.v ps))))
+    (r <==> Some? ps) /\ (r ==> (aff_point_inv h1 res /\ as_aff_point_nat_inv h1 res == Some?.v ps))))
 
 
-val load_point_vartime: res:point -> b:lbuffer uint8 64ul -> Stack bool
+val load_point_vartime: {| cp:S.curve_params |} -> res:point -> b:lbuffer uint8 (2ul *. size cp.bytes) -> Stack bool
   (requires fun h ->
     live h res /\ live h b /\ disjoint res b)
   (ensures  fun h0 r h1 -> modifies (loc res) h0 h1 /\
@@ -251,7 +262,7 @@ val load_point_vartime: res:point -> b:lbuffer uint8 64ul -> Stack bool
       from_mont_point (as_point_nat h1 res) == Some?.v ps))))
 
 
-val aff_point_decompress_vartime (x y:felem) (s:lbuffer uint8 33ul) : Stack bool
+val aff_point_decompress_vartime {| S.curve_params |} (x y:felem) (s:lbuffer uint8 (1ul +. (size S.bytes))) : Stack bool
   (requires fun h ->
     live h x /\ live h y /\ live h s /\
     disjoint x y /\ disjoint x s /\ disjoint y s)
