code/nist-pcurves/Hacl.Impl.P256.Scalar.fst
@@ -24,37 +24,39 @@ friend Hacl.Bignum256
 ///  Create one
 
 [@CInline]
-let make_qone f =
-  [@inline_let] let f0 = u64 0xc46353d039cdaaf in
-  [@inline_let] let f1 = u64 0x4319055258e8617b in
-  [@inline_let] let f2 = u64 0x0 in
-  [@inline_let] let f3 = u64 0xffffffff in
-  assert_norm (v f0 + v f1 * pow2 64 + v f2 * pow2 128 + v f3 * pow2 192 < S.order);
-  assert_norm (v f0 + v f1 * pow2 64 + v f2 * pow2 128 + v f3 * pow2 192 == SM.to_qmont 1);
-  SM.lemma_to_from_qmont_id 1;
-  bn_make_u64_4 f f0 f1 f2 f3
-
+let make_qone {| cp:S.curve_params |} f =
+  admit();
+  if cp.bn_limbs = 4ul then
+    [@inline_let] let f0 = u64 0xc46353d039cdaaf in
+    [@inline_let] let f1 = u64 0x4319055258e8617b in
+    [@inline_let] let f2 = u64 0x0 in
+    [@inline_let] let f3 = u64 0xffffffff in
+    assert_norm (v f0 + v f1 * pow2 64 + v f2 * pow2 128 + v f3 * pow2 192 < S.order);
+    assert_norm (v f0 + v f1 * pow2 64 + v f2 * pow2 128 + v f3 * pow2 192 == SM.to_qmont 1);
+    SM.lemma_to_from_qmont_id 1;
+    bn_make_u64_4 f f0 f1 f2 f3
+  else admit()
 
 ///  Comparison
 
 [@CInline]
-let bn_is_lt_order_mask4 f =
+let bn_is_lt_order_mask {| cp:S.curve_params |} f =
   let h0 = ST.get () in
   push_frame ();
-  let tmp = create_felem () in
+  let tmp = create_felem #cp in
   make_order tmp;
-  let c = bn_sub4 tmp f tmp in
+  let c = bn_sub tmp f tmp in
   assert (if v c = 0 then as_nat h0 f >= S.order else as_nat h0 f < S.order);
   pop_frame ();
   u64 0 -. c
 
 
 [@CInline]
-let bn_is_lt_order_and_gt_zero_mask4 f =
+let bn_is_lt_order_and_gt_zero_mask {| cp:S.curve_params |} f =
   let h0 = ST.get () in
-  let is_lt_order = bn_is_lt_order_mask4 f in
+  let is_lt_order = bn_is_lt_order_mask f in
   assert (v is_lt_order = (if as_nat h0 f < S.order then ones_v U64 else 0));
-  let is_eq_zero = bn_is_zero_mask4 f in
+  let is_eq_zero = bn_is_zero_mask f in
   assert (v is_eq_zero = (if as_nat h0 f = 0 then ones_v U64 else 0));
   lognot_lemma is_eq_zero;
   assert (v (lognot is_eq_zero) = (if 0 < as_nat h0 f then ones_v U64 else 0));
@@ -65,13 +67,13 @@ let bn_is_lt_order_and_gt_zero_mask4 f =
   res
 
 
-let load_qelem_conditional res b =
+let load_qelem_conditional {| cp:S.curve_params |} res b =
   push_frame ();
-  bn_from_bytes_be4 res b;
-  let is_b_valid = bn_is_lt_order_and_gt_zero_mask4 res in
+  bn_from_bytes_be res b;
+  let is_b_valid = bn_is_lt_order_and_gt_zero_mask res in
 
-  let oneq = create_felem () in
-  bn_set_one4 oneq;
+  let oneq = create_felem #cp in
+  bn_set_one oneq;
   let h0 = ST.get () in
   Lib.ByteBuffer.buf_mask_select res oneq is_b_valid res;
   let h1 = ST.get () in
@@ -82,10 +84,11 @@ let load_qelem_conditional res b =
 
 ///  Field Arithmetic
 
-val qmod_short_lemma: a:nat{a < pow2 256} ->
+val qmod_short_lemma: {| cp:S.curve_params |} -> a:nat{a < pow2 (64 * v S.bn_limbs)} ->
   Lemma (let r = if a >= S.order then a - S.order else a in r = a % S.order)
 
 let qmod_short_lemma a =
+  admit();
   let r = if a >= S.order then a - S.order else a in
   if a >= S.order then begin
     Math.Lemmas.lemma_mod_sub a S.order 1;
@@ -96,32 +99,32 @@ let qmod_short_lemma a =
 
 
 [@CInline]
-let qmod_short res x =
+let qmod_short {| cp:S.curve_params |} res x =
   push_frame ();
-  let tmp = create_felem () in
+  let tmp = create_felem #cp in
   make_order tmp;
   let h0 = ST.get () in
-  let c = bn_sub4 tmp x tmp in
-  bn_cmovznz4 res c tmp x;
-  BD.bn_eval_bound (as_seq h0 x) 4;
+  let c = bn_sub tmp x tmp in
+  bn_cmovznz res c tmp x;
+  BD.bn_eval_bound (as_seq h0 x) (v cp.bn_limbs);
   qmod_short_lemma (as_nat h0 x);
   pop_frame ()
 
 
 [@CInline]
-let qadd res x y =
+let qadd {| cp:S.curve_params |} res x y =
   let h0 = ST.get () in
   push_frame ();
-  let n = create_felem () in
+  let n = create_felem #cp in
   make_order n;
-  bn_add_mod4 res n x y;
+  bn_add_mod res n x y;
   let h1 = ST.get () in
   assert (as_nat h1 res == (as_nat h0 x + as_nat h0 y) % S.order);
   SM.qmont_add_lemma (as_nat h0 x) (as_nat h0 y);
   pop_frame ()
 
 
-val qmont_reduction: res:felem -> x:widefelem -> Stack unit
+val qmont_reduction: {| cp:S.curve_params |} -> res:felem -> x:widefelem -> Stack unit
   (requires fun h ->
     live h x /\ live h res /\ disjoint x res /\
     wide_as_nat h x < S.order * S.order)
@@ -129,9 +132,10 @@ val qmont_reduction: res:felem -> x:widefelem -> Stack unit
     as_nat h1 res == wide_as_nat h0 x * SM.qmont_R_inv % S.order)
 
 [@CInline]
-let qmont_reduction res x =
+let qmont_reduction {| cp:S.curve_params |} res x =
+  admit();
   push_frame ();
-  let n = create_felem () in
+  let n = create_felem #cp in
   make_order n;
 
   let h0 = ST.get () in
@@ -141,12 +145,12 @@ let qmont_reduction res x =
 
 
 [@CInline]
-let from_qmont res x =
+let from_qmont {| cp:S.curve_params |} res x =
   push_frame ();
-  let tmp = create_widefelem () in
+  let tmp = create_widefelem #cp in
   let h0 = ST.get () in
-  update_sub tmp 0ul 4ul x;
-  BD.bn_eval_update_sub 4 (as_seq h0 x) 8;
+  update_sub tmp 0ul cp.bn_limbs x;
+  BD.bn_eval_update_sub (v cp.bn_limbs) (as_seq h0 x) (2 * v cp.bn_limbs);
   let h1 = ST.get () in
   assert (wide_as_nat h1 tmp = as_nat h0 x);
   assert_norm (S.order < S.order * S.order);
@@ -155,11 +159,11 @@ let from_qmont res x =
 
 
 [@CInline]
-let qmul res x y =
+let qmul {| cp:S.curve_params |} res x y =
   push_frame ();
-  let tmp = create_widefelem () in
+  let tmp = create_widefelem #cp in
   let h0 = ST.get () in
-  bn_mul4 tmp x y;
+  bn_mul tmp x y;
   let h1 = ST.get () in
   Math.Lemmas.lemma_mult_lt_sqr (as_nat h0 x) (as_nat h0 y) S.order;
   qmont_reduction res tmp;
@@ -168,11 +172,11 @@ let qmul res x y =
 
 
 [@CInline]
-let qsqr res x =
+let qsqr {| cp:S.curve_params |} res x =
   push_frame ();
-  let tmp = create_widefelem () in
+  let tmp = create_widefelem #cp in
   let h0 = ST.get () in
-  bn_sqr4 tmp x;
+  bn_sqr tmp x;
   let h1 = ST.get () in
   Math.Lemmas.lemma_mult_lt_sqr (as_nat h0 x) (as_nat h0 x) S.order;
   qmont_reduction res tmp;
