code/nist-pcurves/Hacl.Spec.P256.PrecompTable.fst
@@ -29,28 +29,31 @@ let create4_lemma x0 x1 x2 x3 =
 //-----------------------------------
 
 noextract
-let list_as_felem4 (f:felem_list) : lseq uint64 4 =
-  Seq.seq_of_list f <: lseq uint64 4
+let list_as_felem {| cp:S.curve_params |} (f:felem_list) : lseq uint64 (v cp.bn_limbs) =
+  Seq.seq_of_list f <: lseq uint64 (v cp.bn_limbs)
 
 
-val felem_to_list_lemma_eval: x:S.felem ->
-  Lemma (BD.bn_v (list_as_felem4 (felem_to_list x)) == x)
+val felem_to_list_lemma_eval: {| cp:S.curve_params |} -> x:S.felem ->
+  Lemma (BD.bn_v (list_as_felem (felem_to_list x)) == x)
 
-let felem_to_list_lemma_eval x =
-  let x0 = x % pow2 64 in
-  let x1 = x / pow2 64 % pow2 64 in
-  let x2 = x / pow2 128 % pow2 64 in
-  let x3 = x / pow2 192 % pow2 64 in
-  let bn_x = list_as_felem4 (felem_to_list x) in
-  create4_lemma (u64 x0) (u64 x1) (u64 x2) (u64 x3);
-  assert (v bn_x.[0] == x0 /\ v bn_x.[1] == x1 /\ v bn_x.[2] == x2 /\ v bn_x.[3] == x3);
-  Hacl.Impl.P256.Bignum.bn_v_is_as_nat bn_x;
-  assert (BD.bn_v bn_x = x0 + x1 * pow2 64 + x2 * pow2 128 + x3 * pow2 192);
-  Hacl.Spec.PrecompBaseTable256.lemma_decompose_nat256_as_four_u64 x
+let felem_to_list_lemma_eval {| cp:S.curve_params |} x =
+  if cp.bn_limbs = 4ul then (
+    assume (cp.bits == 256);
+    let x0 = x % pow2 64 in
+    let x1 = x / pow2 64 % pow2 64 in
+    let x2 = x / pow2 128 % pow2 64 in
+    let x3 = x / pow2 192 % pow2 64 in
+    let bn_x = list_as_felem (felem_to_list x) in
+    create4_lemma (u64 x0) (u64 x1) (u64 x2) (u64 x3);
+      assert (v bn_x.[0] == x0 /\ v bn_x.[1] == x1 /\ v bn_x.[2] == x2 /\ v bn_x.[3] == x3);
+    Hacl.Impl.P256.Bignum.bn_v_is_as_nat4 bn_x;
+      assert (BD.bn_v bn_x = x0 + x1 * pow2 64 + x2 * pow2 128 + x3 * pow2 192);
+    Hacl.Spec.PrecompBaseTable256.lemma_decompose_nat256_as_four_u64 x)
+  else admit()
 
 //--------------------------------------------
 
-val proj_point_to_list_sub: p:S.proj_point -> Lemma
+val proj_point_to_list_sub {| cp:S.curve_params |} : p:S.proj_point -> Lemma
  (let (px, py, pz) = p in
   let pxM = SM.to_mont px in
   let pyM = SM.to_mont py in
@@ -60,15 +63,15 @@ val proj_point_to_list_sub: p:S.proj_point -> Lemma
   let pz_list = felem_to_list pzM in
   let p_list = FL.(px_list @ py_list @ pz_list) in
 
-  let p_lseq = Seq.seq_of_list p_list <: lseq uint64 12 in
-  let px_lseq = Seq.seq_of_list px_list <: lseq uint64 4 in
-  let py_lseq = Seq.seq_of_list py_list <: lseq uint64 4 in
-  let pz_lseq = Seq.seq_of_list pz_list <: lseq uint64 4 in
-  sub p_lseq 0 4 == px_lseq /\
-  sub p_lseq 4 4 == py_lseq /\
-  sub p_lseq 8 4 == pz_lseq)
+  let p_lseq = Seq.seq_of_list p_list <: lseq uint64 (3 * v cp.bn_limbs) in
+  let px_lseq = Seq.seq_of_list px_list <: lseq uint64 (v cp.bn_limbs) in
+  let py_lseq = Seq.seq_of_list py_list <: lseq uint64 (v cp.bn_limbs) in
+  let pz_lseq = Seq.seq_of_list pz_list <: lseq uint64 (v cp.bn_limbs) in
+  sub p_lseq 0 (v cp.bn_limbs) == px_lseq /\
+  sub p_lseq (v cp.bn_limbs) (v cp.bn_limbs) == py_lseq /\
+  sub p_lseq (2 * v cp.bn_limbs) (v cp.bn_limbs) == pz_lseq)
 
-let proj_point_to_list_sub p =
+let proj_point_to_list_sub {| cp:S.curve_params |} p =
   let (px, py, pz) = p in
   let pxM = SM.to_mont px in
   let pyM = SM.to_mont py in
@@ -82,10 +85,10 @@ let proj_point_to_list_sub p =
   SPT.seq_of_list_append_lemma FL.(px_list @ py_list) pz_list
 
 
-val proj_point_to_list_fits: p:S.proj_point ->
+val proj_point_to_list_fits {| cp:S.curve_params |} : p:S.proj_point ->
   Lemma (point_inv_list (proj_point_to_list p))
 
-let proj_point_to_list_fits p =
+let proj_point_to_list_fits {| cp:S.curve_params |} p =
   let (px, py, pz) = p in
   let pxM = SM.to_mont px in
   let pyM = SM.to_mont py in
@@ -97,8 +100,8 @@ let proj_point_to_list_fits p =
   felem_to_list_lemma_eval pzM
 
 
-val proj_point_to_list_eval: p:S.proj_point ->
-  Lemma (point_eval_list (proj_point_to_list p) == p)
+val proj_point_to_list_eval: {| cp:S.curve_params |} -> p:S.proj_point ->
+  Lemma (point_eval_list (proj_point_to_list p) == p) 
 
 let proj_point_to_list_eval p =
   let (px, py, pz) = p in
