code/nist-pcurves/Hacl.Spec.P256.PrecompTable.fsti
@@ -4,7 +4,7 @@ open FStar.Mul
 open Lib.IntTypes
 open Lib.Sequence
 
-//open Hacl.Impl.P256.Point
+open Hacl.Impl.P256.Point
 
 module S = Spec.P256
 module SM = Hacl.Spec.P256.Montgomery
@@ -16,19 +16,23 @@ unfold
 let create4 (x0 x1 x2 x3:uint64) : list uint64 = [x0; x1; x2; x3]
 
 inline_for_extraction noextract
-let felem_list = x:list uint64{FL.length x == 4}
+let felem_list {| cp:S.curve_params |} =
+    x:list uint64{FL.length x == v cp.bn_limbs}
 inline_for_extraction noextract
-let point_list = x:list uint64{FL.length x == 12}
+let point_list {| cp:S.curve_params |} =
+    x:list uint64{FL.length x == 3 * v cp.bn_limbs}
 
 inline_for_extraction noextract
-let felem_to_list {| S.curve_params |} (x:S.felem) : felem_list =
-  [@inline_let] let x0 = x % pow2 64 in
-  [@inline_let] let x1 = x / pow2 64 % pow2 64 in
-  [@inline_let] let x2 = x / pow2 128 % pow2 64 in
-  [@inline_let] let x3 = x / pow2 192 % pow2 64 in
-  [@inline_let] let r = create4 (u64 x0) (u64 x1) (u64 x2) (u64 x3) in
-  assert_norm (FL.length r = 4);
-  r
+let felem_to_list {| cp:S.curve_params |} (x:S.felem) : felem_list =
+  if cp.bn_limbs = 4ul then 
+    [@inline_let] let x0 = x % pow2 64 in
+    [@inline_let] let x1 = x / pow2 64 % pow2 64 in
+    [@inline_let] let x2 = x / pow2 128 % pow2 64 in
+    [@inline_let] let x3 = x / pow2 192 % pow2 64 in
+    [@inline_let] let r = create4 (u64 x0) (u64 x1) (u64 x2) (u64 x3) in
+    assert_norm (FL.length r = 4);
+    r
+  else admit()
 
 inline_for_extraction noextract
 let proj_point_to_list {| S.curve_params |} (p:S.proj_point) : point_list =
@@ -38,15 +42,17 @@ let proj_point_to_list {| S.curve_params |} (p:S.proj_point) : point_list =
   [@inline_let] let pzM = SM.to_mont pz in
   FL.(felem_to_list pxM @ felem_to_list pyM @ felem_to_list pzM)
 
+
 inline_for_extraction noextract
-let point_inv_list {| S.curve_params |} (p:point_list) =
-  let x = Seq.seq_of_list p <: lseq uint64 12 in
+let point_inv_list {| cp:S.curve_params |} (p:point_list) =
+  let x = Seq.seq_of_list p <: lseq uint64 (3 * v cp.bn_limbs) in
   point_inv_seq x
 
 noextract
-let point_eval_list (p:point_list) =
-  let x = Seq.seq_of_list p <: lseq uint64 12 in
+let point_eval_list {| cp: S.curve_params |} (p:point_list) =
+  let x = Seq.seq_of_list p <: lseq uint64 (3 * v cp.bn_limbs)  in
   from_mont_point (as_point_nat_seq x)
+    
 
-val proj_point_to_list_lemma: p:S.proj_point ->
+val proj_point_to_list_lemma {| S.curve_params |} : p:S.proj_point ->
   Lemma (point_inv_list (proj_point_to_list p) /\ point_eval_list (proj_point_to_list p) == p)
