code/nist-pcurves/Hacl.Impl.P256.Compression.fsti
@@ -13,7 +13,8 @@ module S = Spec.P256
 #set-options "--z3rlimit 30 --fuel 0 --ifuel 0"
 
 inline_for_extraction noextract
-val uncompressed_to_raw: pk:lbuffer uint8 65ul -> pk_raw:lbuffer uint8 64ul -> Stack bool
+val uncompressed_to_raw: {| cp:S.curve_params |} -> pk:lbuffer uint8 (1ul +. 2ul *. size cp.bytes) ->
+                         pk_raw:lbuffer uint8 (2ul *. size cp.bytes) -> Stack bool
   (requires fun h -> live h pk /\ live h pk_raw /\ disjoint pk pk_raw)
   (ensures fun h0 b h1 -> modifies (loc pk_raw) h0 h1 /\
     (b <==> Some? (S.pk_uncompressed_to_raw (as_seq h0 pk))) /\
@@ -21,7 +22,8 @@ val uncompressed_to_raw: pk:lbuffer uint8 65ul -> pk_raw:lbuffer uint8 64ul -> S
 
 
 inline_for_extraction noextract
-val compressed_to_raw: pk:lbuffer uint8 33ul -> pk_raw:lbuffer uint8 64ul -> Stack bool
+val compressed_to_raw: {| cp:S.curve_params |} -> pk:lbuffer uint8 (1ul +. size cp.bytes) ->
+                       pk_raw:lbuffer uint8 (2ul *. size cp.bytes) -> Stack bool
   (requires fun h -> live h pk /\ live h pk_raw /\ disjoint pk pk_raw)
   (ensures  fun h0 b h1 -> modifies (loc pk_raw) h0 h1 /\
     (b <==> Some? (S.pk_compressed_to_raw (as_seq h0 pk))) /\
@@ -29,14 +31,16 @@ val compressed_to_raw: pk:lbuffer uint8 33ul -> pk_raw:lbuffer uint8 64ul -> Sta
 
 
 inline_for_extraction noextract
-val raw_to_uncompressed: pk_raw:lbuffer uint8 64ul -> pk:lbuffer uint8 65ul -> Stack unit
+val raw_to_uncompressed: {| cp:S.curve_params |} -> pk_raw:lbuffer uint8 (2ul *. size cp.bytes) ->
+                         pk:lbuffer uint8 (1ul +. 2ul *. size cp.bytes) -> Stack unit
   (requires fun h -> live h pk /\ live h pk_raw /\ disjoint pk pk_raw)
   (ensures fun h0 _ h1 -> modifies (loc pk) h0 h1 /\
     as_seq h1 pk == S.pk_uncompressed_from_raw (as_seq h0 pk_raw))
 
 
 inline_for_extraction noextract
-val raw_to_compressed: pk_raw:lbuffer uint8 64ul -> pk:lbuffer uint8 33ul -> Stack unit
+val raw_to_compressed: {| cp:S.curve_params |} -> pk_raw:lbuffer uint8 (2ul *. size cp.bytes) ->
+                       pk:lbuffer uint8 (1ul +. size cp.bytes) -> Stack unit
   (requires fun h -> live h pk /\ live h pk_raw /\ disjoint pk pk_raw)
   (ensures  fun h0 _ h1 -> modifies (loc pk) h0 h1 /\
     as_seq h1 pk == S.pk_compressed_from_raw (as_seq h0 pk_raw))
