code/nist-pcurves/Hacl.Impl.P256.Scalar.fsti
@@ -16,11 +16,11 @@ module BSeq = Lib.ByteSequence
 
 #set-options "--z3rlimit 30 --fuel 0 --ifuel 0"
 
-let qmont_as_nat (h:mem) (a:felem) = SM.from_qmont (as_nat h a)
+let qmont_as_nat {| c:S.curve_params |} (h:mem) (a:felem) = SM.from_qmont (as_nat h a)
 
 ///  Create one
 
-val make_qone: f:felem -> Stack unit
+val make_qone: {| cp:S.curve_params |} -> f:felem -> Stack unit
   (requires fun h -> live h f)
   (ensures  fun h0 _ h1 -> modifies (loc f) h0 h1 /\
     as_nat h1 f < S.order /\
@@ -29,20 +29,20 @@ val make_qone: f:felem -> Stack unit
 
 ///  Comparison
 
-val bn_is_lt_order_mask4: f:felem -> Stack uint64
+val bn_is_lt_order_mask: {| cp:S.curve_params |} -> f:felem -> Stack uint64
   (requires fun h -> live h f)
   (ensures  fun h0 r h1 -> modifies0 h0 h1 /\
     (if as_nat h0 f < S.order then v r = ones_v U64 else v r = 0))
 
 
-val bn_is_lt_order_and_gt_zero_mask4: f:felem -> Stack uint64
+val bn_is_lt_order_and_gt_zero_mask: {| cp:S.curve_params |} -> f:felem -> Stack uint64
   (requires fun h -> live h f)
   (ensures  fun h0 r h1 -> modifies0 h0 h1 /\
     (if 0 < as_nat h0 f && as_nat h0 f < S.order then v r = ones_v U64 else v r = 0))
 
 
 inline_for_extraction noextract
-val load_qelem_conditional: res:felem -> b:lbuffer uint8 32ul -> Stack uint64
+val load_qelem_conditional: {| cp:S.curve_params |} -> res:felem -> b:lbuffer uint8 (size cp.bytes) -> Stack uint64
   (requires fun h ->
     live h res /\ live h b /\ disjoint res b)
   (ensures fun h0 m h1 -> modifies (loc res) h0 h1 /\
@@ -54,14 +54,14 @@ val load_qelem_conditional: res:felem -> b:lbuffer uint8 32ul -> Stack uint64
 
 ///  Field Arithmetic
 
-val qmod_short: res:felem -> x:felem -> Stack unit
+val qmod_short: {| cp:S.curve_params |} -> res:felem -> x:felem -> Stack unit
   (requires fun h ->
     live h x /\ live h res /\ eq_or_disjoint x res)
   (ensures fun h0 _ h1 -> modifies (loc res) h0 h1 /\
     as_nat h1 res == as_nat h0 x % S.order)
 
 
-val qadd: res:felem -> x:felem -> y:felem -> Stack unit
+val qadd: {| cp:S.curve_params |} -> res:felem -> x:felem -> y:felem -> Stack unit
   (requires fun h ->
     live h x /\ live h y /\ live h res /\
     eq_or_disjoint x y /\ eq_or_disjoint x res /\ eq_or_disjoint y res /\
@@ -71,7 +71,7 @@ val qadd: res:felem -> x:felem -> y:felem -> Stack unit
     qmont_as_nat h1 res == S.qadd (qmont_as_nat h0 x) (qmont_as_nat h0 y))
 
 
-val from_qmont: res:felem -> x:felem -> Stack unit
+val from_qmont: {| cp:S.curve_params |} -> res:felem -> x:felem -> Stack unit
   (requires fun h ->
     live h x /\ live h res /\ eq_or_disjoint x res /\
     as_nat h x < S.order)
@@ -80,7 +80,7 @@ val from_qmont: res:felem -> x:felem -> Stack unit
     as_nat h1 res == qmont_as_nat h0 x)
 
 
-val qmul: res:felem -> x:felem -> y:felem -> Stack unit
+val qmul: {| cp:S.curve_params |} -> res:felem -> x:felem -> y:felem -> Stack unit
   (requires fun h ->
     live h x /\ live h y /\ live h res /\
     eq_or_disjoint x y /\ eq_or_disjoint x res /\ eq_or_disjoint y res /\
@@ -90,7 +90,7 @@ val qmul: res:felem -> x:felem -> y:felem -> Stack unit
     qmont_as_nat h1 res = S.qmul (qmont_as_nat h0 x) (qmont_as_nat h0 y))
 
 
-val qsqr: res:felem -> x:felem -> Stack unit
+val qsqr: {| cp:S.curve_params |} -> res:felem -> x:felem -> Stack unit
   (requires fun h ->
     live h x /\ live h res /\ eq_or_disjoint x res /\
     as_nat h x < S.order)
